FokkerChallenge/TwoVarsAreNotEnough/Basic.lean
@@ -1,7 +1,21 @@
 import Cslib.Languages.LambdaCalculus.LocallyNameless.Untyped.Basic
 import Cslib.Languages.LambdaCalculus.LocallyNameless.Untyped.LcAt
+import Cslib.Languages.LambdaCalculus.LocallyNameless.Untyped.ListFullBeta
+import Cslib.Languages.LambdaCalculus.LocallyNameless.Untyped.FullBetaConfluence
+import Cslib.Languages.LambdaCalculus.LocallyNameless.Untyped.FullBetaEtaConfluence
+import Cslib.Languages.LambdaCalculus.LocallyNameless.Untyped.LeftmostReduction
 import Cslib.Foundations.Data.HasFresh
 import FokkerChallenge.Basic
+import FokkerChallenge.FamousCombinator
+import FokkerChallenge.EnhancedCslib.Basic
+import FokkerChallenge.EnhancedCslib.FlipApp
+import FokkerChallenge.EnhancedCslib.LeftMost
+import FokkerChallenge.EnhancedCslib.BetaNormalForm
+import FokkerChallenge.EnhancedCslib.Closedunderapp
+import FokkerChallenge.EnhancedCslib.List
+import FokkerChallenge.EnhancedCslib.HeadNFSpineEta
+import FokkerChallenge.EnhancedCslib.ReflTransGenWithSteps
+import FokkerChallenge.EnhancedCslib.HeadRed
 import Mathlib.Data.Finset.Basic
 import Mathlib.Data.Finset.Insert
 import Mathlib.Data.Finset.Union
@@ -13,22 +27,23 @@ namespace LambdaCalculus.LocallyNameless.Untyped.Term
 @[scoped grind =]
 def two_vars_are_enough: Term String → Bool
   | Term.bvar n => n < 2
-  | Term.fvar _ => true
+  | Term.fvar _ => false
   | Term.abs (Term.abs t) => two_vars_are_enough t
   | Term.app t1 t2 => two_vars_are_enough t1 && two_vars_are_enough t2
   | _ => false
 
 @[scoped grind]
-theorem two_vars_are_enough_lcat {t} (g : two_vars_are_enough t) : LcAt 2 t := by
+theorem two_vars_are_enough_lc {t} (g : two_vars_are_enough t) : t.abs.abs.LC := by
+  rw [<- lcAt_iff_LC]
   induction h : t.fokker_size using Nat.strong_induction_on generalizing t with
   | h n ih => cases t with
-  | fvar _ => grind
-  | bvar n => grind
-  | app t1 t2 => grind
+  | fvar => grind
+  | bvar => grind
+  | app => grind
   | abs t => cases t with
-    | bvar _ => grind
-    | fvar _ => grind
-    | app _ _ => grind
+    | bvar => grind
+    | fvar => grind
+    | app => grind
     | abs t =>  specialize @ih _ ?_ t ?_ rfl
                 grind
                 grind
@@ -36,14 +51,32 @@ theorem two_vars_are_enough_lcat {t} (g : two_vars_are_enough t) : LcAt 2 t := b
                 unfold LcAt
                 refine lcAt_le _ _ _ (by omega) ih
 
-@[scoped grind]
-theorem two_vars_are_enough_lc {t} (g : two_vars_are_enough t) : t.abs.abs.LC := by
-  rw [<- lcAt_iff_LC]
-  unfold LcAt
-  unfold LcAt
-  simp
-  apply two_vars_are_enough_lcat g
+theorem two_vars_are_enough_depth {M N1 N2: Term String}
+  (hm : M.two_vars_are_enough)
+  (h1 : N1.LC) (h2 : N2.LC) :
+  M⟦1 ↝ N1⟧⟦0 ↝ N2⟧.depth <= M.depth.max (N1.depth.max N2.depth) := by
+  induction h : M.fokker_size using Nat.strong_induction_on generalizing M with | h n ih =>
+  cases M with
+  | fvar _ => grind
+  | bvar _ => grind
+  | abs M => cases M <;> grind
+  | app a b =>
+      have := @ih _ (by grind) a (by grind) rfl
+      have := @ih _ (by grind) b (by grind) rfl
+      rw [openRec_app, openRec_app]
+      grind
 
+@[scoped grind =]
+theorem two_vars_are_enough_fv {t} (h: two_vars_are_enough t) : t.fv = ∅ := by
+  induction h : t.fokker_size using Nat.strong_induction_on generalizing t with
+    | h n _ => cases t with
+  | bvar _ => grind
+  | fvar _ => grind
+  | app _ _ => grind
+  | abs t => induction t with grind
+
+
+/-
 theorem two_vars_are_enough_openRec {i x t} (g : two_vars_are_enough t) :
   two_vars_are_enough (t⟦i ↝ fvar x⟧) := by
   induction h : t.fokker_size using Nat.strong_induction_on generalizing t with
@@ -52,97 +85,528 @@ theorem two_vars_are_enough_openRec {i x t} (g : two_vars_are_enough t) :
   | fvar _ => grind
   | app _ _ => grind
   | abs t => cases t with grind
+-/
 
 @[scoped grind =]
-def subterms : Term String -> Finset (Term String)
-  | Term.bvar _ => ∅
-  | Term.fvar _ => ∅
-  | Term.abs (Term.abs t) => insert t.abs.abs (subterms t)
-  | Term.abs _ => ∅
-  | Term.app t1 t2 => subterms t1 ∪ subterms t2
+def abs_two_vars_are_enough: Term String → Bool
+  | Term.abs (Term.abs t) => two_vars_are_enough t
+  | _ => false
+
+theorem abs_two_vars_are_enough_weak {t} (h: abs_two_vars_are_enough t) :
+  t.two_vars_are_enough := by
+  unfold abs_two_vars_are_enough at h
+  grind
+
+@[scoped grind =]
+theorem abs_two_vars_are_enough_fv {t} (h: abs_two_vars_are_enough t) : t.fv = ∅ :=
+  two_vars_are_enough_fv (abs_two_vars_are_enough_weak h)
 
 @[scoped grind]
-theorem subterms_size {t} :
-    ∀ s ∈ subterms t, s.fokker_size <= t.fokker_size := by
-  induction h : t.fokker_size using Nat.strong_induction_on generalizing t with
-  | h n _ => cases t with
-  | bvar _ => grind
+theorem abs_two_vars_are_enough_lc {t} (h: abs_two_vars_are_enough t) : t.LC := by
+  unfold abs_two_vars_are_enough at h
+  split at h <;> grind
+
+
+/-
+@[scoped grind]
+inductive GenFinset (atoms: Finset (Term String)) : Term String → Prop where
+  | base : ∀ atom ∈ atoms, GenFinset atoms atom
+  | app {M N}  : GenFinset atoms M → GenFinset atoms N → GenFinset atoms (app M N)
+
+@[scoped grind]
+theorem genFinset_lc (fs : Finset (Term String))
+  (h2 :  ∀ t ∈ fs, t.LC) {t} (ht: GenFinset fs t) : t.LC := by
+  induction ht with grind
+
+@[scoped grind]
+theorem genFinset_fv (fs : Finset (Term String))
+  (hfv : ∀ t ∈ fs, t.fv = ∅)
+   {t} (ht: GenFinset fs t) : t.fv = ∅ := by
+  induction ht with grind
+
+theorem gen_abs_2_vars_are_enough {atom M : Term String} (h : Gen atom M) (g : atom.abs_two_vars_are_enough):
+  GenFinset atom.subterms M := by
+  induction h with
+  | base => apply GenFinset.base
+            unfold abs_two_vars_are_enough at g
+            grind
+  | app _ _ _ _ => grind
+
+
+theorem genFinset_open2 (fs : Finset (Term String))
+  (h2 :  ∀ t ∈ fs, t.LC)
+  {x : Term String}
+  (hx : x.two_vars_are_enough)
+  (hsubset : x.subterms ⊆ fs)
+  (hfv : x.fv = ∅) :
+  ∀ y z, GenFinset fs y -> GenFinset fs z -> GenFinset fs (x⟦1 ↝ y⟧⟦0 ↝ z⟧) := by
+  induction h : x.fokker_size using Nat.strong_induction_on generalizing x with
+  | h n ih => cases x with intros y z hy hz
+  | bvar n => clear ih
+              rw [openRec_bvar]
+              split
+              . rw [open_lc] <;> grind
+              . grind
+  | fvar _ => simp at hfv
+  | app _ _ =>  rw [openRec_app]
+                apply GenFinset.app <;> apply ih
+                any_goals rfl
+                all_goals grind
+  | abs t => cases t with
+    | bvar _ => clear ih; grind
+    | fvar _ => clear ih; grind
+    | app _ _ => clear ih; grind
+    | abs t =>  rw [open_lc, open_lc]
+                · apply GenFinset.base
+                  grind
+                · grind
+                · rw [open_lc] <;> grind
+
+theorem genFinset_list (fs : Finset (Term String))
+  {f} {l : List (Term String)}
+  (ht: GenFinset fs f)
+  (hl : ∀ x ∈ l, GenFinset fs x) : GenFinset fs (l.foldl Term.app f) := by
+  induction l generalizing f with grind
+-/
+
+
+axiom BetaAt.step_fv {M N: Term String} {i} : BetaAt i M N -> N.fv ⊆ M.fv
+
+
+@[scoped grind]
+def fvar_or_combinator (a: Term String) : Prop :=  a.IsFvar \/ a.abs_two_vars_are_enough
+
+theorem two_vars_are_enough_openRec {t N1 N0}
+  (g : two_vars_are_enough t)
+  (h1: ClosedUnderApp fvar_or_combinator N1)
+  (h2: ClosedUnderApp fvar_or_combinator N0) :
+  ClosedUnderApp fvar_or_combinator (t⟦1 ↝ N1⟧⟦0 ↝ N0⟧) := by
+  induction t with
   | fvar _ => grind
   | app _ _ => grind
-  | abs t => cases t with grind
+  | abs t => cases t <;> grind
+  | bvar a => unfold two_vars_are_enough at g
+              have h : a = 0 \/ a = 1 := by grind
+              cases h <;> subst_vars
+              . grind
+              . simp [openRec]
+                rw [open_lc] <;> grind
 
-theorem subterms_gen {t M} (h : Gen t M) : t.subterms = M.subterms := by
-  induction h with grind
+/-
+theorem recursive_app_fvar_fvar_or_combinator {i y M}
+  (hm : ClosedUnderApp fvar_or_combinator M):
+  ClosedUnderApp fvar_or_combinator ((fun a => a.app (fvar y))^[i] (M)) := by
+  induction i generalizing M with (simp; grind)
+-/
 
 
 @[scoped grind]
-theorem subterms_two_vars_are_enough {t} (h : two_vars_are_enough t) :
-    ∀ s ∈ subterms t, two_vars_are_enough s := by
-    induction h : t.fokker_size using Nat.strong_induction_on generalizing t with
-    | h n _ => cases t with
-      | bvar _ => grind
-      | fvar _ => grind
-      | app _ _ => grind
-      | abs t => cases t with grind
+def contain_x (M : Term String) := ∀ Y, M ↠βηᶠ Y -> "x" ∈ Y.fv
 
-theorem subterms_preserved_under_openRec {x i t} (h : two_vars_are_enough t) :
-    t.subterms = t⟦i ↝ fvar x⟧.subterms := by
-    induction h : t.fokker_size using Nat.strong_induction_on generalizing t with
-    | h n _ => cases t with
+theorem beta_eta_nf_contain_x {M N : Term String}
+  (steps : M ↠βηᶠ N)
+  (h : Relation.Normal FullBetaEta N)
+  (hn : "x" ∈ N.fv) : contain_x M  := by
+    intros t ht
+    obtain ⟨Z, hz1, hz2⟩ := confluent_beta_eta ht steps
+    have := Relation.Normal.reflTransGen_eq h hz2
+    subst_vars
+    apply FullBetaEta.steps_fv at hz1
+    apply hz1
+    grind
+
+theorem beta_eta_spline_contain_x {Ns : List _} {M : Term String}
+  (steps : M ↠βηᶠ (Ns.foldl app (fvar "x"))) : contain_x M  := by
+    intros t ht
+    obtain ⟨Z, hz1, hz2⟩ := confluent_beta_eta ht steps
+    obtain ⟨l, _, _⟩ := beta_eta_steps_preserve_fvar_apps hz2
+    subst_vars
+    apply FullBetaEta.steps_fv at hz1
+    apply hz1
+    rw [multiapp_fv]
+    grind [union_foldl]
+
+
+/-
+theorem HeadReduction2.head_nf_exists {M : Term String} {x : String} {l : List (Term String)}
+  (hm : ClosedUnderApp fvar_or_combinator M)
+  (h : Relation.ReflTransGen Leftmost M (l.foldl app (fvar x))) :
+  ∃ l' : List _, Relation.ReflTransGen HeadReduction2 M (l'.foldl app (fvar x)) := by
+  generalize heq : List.foldl app (fvar x) l = N
+  rw [heq] at h
+  induction h using Relation.ReflTransGen.head_induction_on₂ generalizing l with
+  | refl => grind
+  | single h => subst_vars
+                exfalso
+                sorry
+  | head₂ h₁ h₂ h ih => induction h₁ using Leftmost.induction_rule with
+    | h_outer M N hm hn => cases hm with
+      | base hm => cases hm <;> grind
+      | app hm _ => cases hm with | base hm => cases hm with
+        | inl hm => grind
+        | inr hm => unfold abs_two_vars_are_enough at hm
+                    split at hm <;> try grind
+                    rename_i heq
+                    cases heq
+                    exfalso
+                    sorry
+    | h_appL h hi _ => sorry
+    | h_appR h hi g _ => sorry
+    | h_abs M M' xs h _ => sorry
+-/
+
+
+
+  /-
+  induction hm generalizing l x with
+  | app _ _ _ _ => sorry
+  | base hm => cases hm with
+    | inl hm => use []
+                simp
+                cases hm
+                generalize heq : List.foldl app (fvar x) l = N
+                rw [heq] at h
+                rcases Relation.ReflTransGen.cases_head h with h|⟨_, g, h2⟩
+                . rcases (List.eq_nil_or_concat' l) with _| ⟨l, b, h⟩
+                  . grind
+                  . subst_vars
+                    rw [List.foldl_concat] at heq
+                    cases heq
+                . generalize hi : 0 = i
+                  unfold Leftmost at g
+                  rw [hi] at g
+                  cases g
+    | inr hm =>
+    unfold abs_two_vars_are_enough at hm
+    split at hm <;> try grind
+    have g :=  Leftmost.steps_isAbs_r h (by grind)
+    rcases (List.eq_nil_or_concat' l) with _| ⟨l, b, h⟩
+    . grind
+    . subst_vars
+      rw [List.foldl_concat] at g
+      cases g
+  -/
+
+/-
+@[scoped grind]
+def P (fs : Finset (Term String)) (t : Term String) : Prop :=
+  let (h, args) := spine t
+  h ∈ fs /\ ∀ x ∈ args, GenFinset fs x
+
+
+@[scoped grind]
+theorem genfinset_P {fs : Finset (Term String)}
+  (h2 :  ∀ t ∈ fs, t.abs_two_vars_are_enough)
+  {t: Term String} :
+  GenFinset fs t <-> P fs t := by
+  constructor
+  . intros h
+    induction h with
+    | base atom _ =>  unfold P
+                      split
+                      rename_i h _ _ _ heq
+                      unfold spine at heq
+                      split at heq <;> grind
+    | app _ _ _ _ => grind
+  . intros h
+    unfold P at h
+    split at h
+    rename_i l _
+    induction t generalizing l with
+    | bvar _ => grind only [spine, GenFinset.base]
+    | fvar _ => grind only [spine, GenFinset.base]
+    | abs _ _ => grind only [spine, GenFinset.base]
+    | app _ _ _ _ => grind only [spine, GenFinset.app, = List.mem_append, = List.mem_cons]
+
+
+@[scoped grind]
+theorem P_fv(fs : Finset (Term String))
+  (hfv : ∀ t ∈ fs, t.fv = ∅)
+  (h2 :  ∀ t ∈ fs, t.abs_two_vars_are_enough)
+   {t} (ht: P fs t) : t.fv = ∅ := by
+  apply genFinset_fv _ hfv
+  rw [genfinset_P]
+  grind
+  grind
+
+
+theorem closedUnderApp_reduce_to_head_apps {M n}
+  (hdepth : M.depth = n)
+  (hm : ClosedUnderApp fvar_or_combinator M)
+  (h : M ↠βᶠ H n) : False:= by
+  induction n using Nat.strong_induction_on generalizing M with | h n ih =>
+  cases n with
+  | zero => cases Relation.ReflTransGen.cases_head h with
+    | inl h => grind
+    | inr h =>  obtain ⟨N, h, _⟩ := h
+                apply FullBeta.depth0 h hdepth
+  | succ n =>
+  have g := Relation.ReflTransGen.trans (FullBeta.redex_app_l_cong (FullBeta.redex_app_l_cong h (LC.fvar "x")) (LC.fvar "y")) H_succ_reduce
+  -- have := closedUnderApp_unroll (by grind) hm
+  sorry
+-/
+
+
+/-
+
+theorem size_dichotomy (t : Term String) :
+    (∀ t', t ↠ℓℓ t' → t'.spine.2.length ≥ 2) ∨
+    (∃ t', t ↠ℓℓ t' ∧ (t'.spine.2.length = 0 ∨ t'.spine.2.length = 1)) := by
+  by_cases h : ∃ t', t ↠ℓℓ t' ∧ t'.spine.2.length ≤ 1
+  · right
+    obtain ⟨t', hstep, hsize⟩ := h
+    exact ⟨t', hstep, by omega⟩
+  · left
+    intro t' hstep
+    by_contra hcon
+    exact h ⟨t', hstep, by omega⟩
+
+lemma step_lc_r {M M' : Term String} (redex : M ⭢ℓℓ M') : LC M -> LC M' := by
+  cases redex
+  grind
+
+@[scoped grind]
+lemma steps_lc_r {M M' : Term String} (redex : M ↠ℓℓ  M') : LC M -> LC M' := by
+  induction redex with grind
+
+@[scoped grind]
+theorem leftmostMulti_to_multi {M N} (h : M ↠ℓℓ N) : M ↠βᶠ N := by
+  induction h with
+  | refl => grind
+  | tail h1 h2 h3 =>  cases h2 with
+
+
+theorem leftmost2_preserves_P_l {fs : Finset (Term String)}
+  (hidempotent : idempotent fs)
+  (h2 :  ∀ t ∈ fs, t.abs_two_vars_are_enough)
+  (hfv : ∀ t ∈ fs, t.fv = ∅)
+  {t t': Term String}
+  (step : t ⭢ℓℓ t')
+  (h5 : P fs t) :
+  P fs t' := by
+  cases step with | base h4 h7 =>
+  rename_i M1 M2 M3 N
+  have h6 := spine_def_2 ((M1.app M2).app M3)
+  generalize hl: ((M1.app M2).app M3).spine.2 = l
+  rw [hl] at h6
+  rw [<- h6] at h4
+  cases l <;> try grind
+  rename_i a l
+  cases l <;> try grind
+  rename_i b l
+  have h7 := h2 ((M1.app M2).app M3).spine.1 (by grind)
+  unfold abs_two_vars_are_enough at h7
+  split at h7 <;> try grind
+  rename_i f heq
+  rw [heq] at h4
+  have : GenFinset fs a := by grind
+  have : GenFinset fs b := by grind
+  have h8 := leftmost_multiapp f.abs a (b::l) (by grind) (by grind)
+  have := BetaAt.unique h8 h4
+  subst N
+  have h8 := leftmost_multiapp (f⟦1 ↝ a⟧) b l (by grind) (by grind)
+  have := BetaAt.unique h8 h7
+  rw [<- genfinset_P]
+  subst t'
+  apply genFinset_list
+  apply genFinset_open2
+  all_goals grind
+
+
+theorem step_leftmost2_preserves_P_r {fs : Finset (Term String)}
+  (hidempotent : idempotent fs)
+  (h2 :  ∀ t ∈ fs, t.abs_two_vars_are_enough)
+  (hfv : ∀ t ∈ fs, t.fv = ∅)
+  {t t': Term String}
+  (step : t ⭢ℓℓ t')
+  (pt: P fs t):
+  P fs t' := by
+  cases t with
+  | bvar _ => grind
+  | fvar _ => grind
+  | abs _ =>  cases step
+  | app M _ => cases M with
     | bvar _ => grind
     | fvar _ => grind
-    | app _ _ => grind
-    | abs t => cases t with grind
+    | app _ _ =>  apply leftmost2_preserves_P_l
+                  any_goals grind
+                  · exact step
+                  · grind
+    | abs _ =>  cases pt with | intro left right =>
+                specialize h2 _ left
+                unfold abs_two_vars_are_enough at h2
+                split at h2 <;> try grind
+                rename_i heq
+                rw [heq] at step
+                cases step
 
-theorem two_vars_are_enough_subterms_lc {t} (h : two_vars_are_enough t) (hlc: t.LC) :
-    ∀ s ∈ subterms t, s.LC := by
-    induction h : t.fokker_size using Nat.strong_induction_on generalizing t with
-    | h n ih => cases t with
-      | bvar _ => grind
-      | fvar _ => grind
-      | app t1 t2 =>  intros s hs
-                      unfold subterms at hs
-                      cases hlc
-                      simp at hs
-                      cases hs
-                      · refine ih t1.fokker_size ?_ ?_ ?_ rfl ?_ ?_
-                        all_goals grind
-                      · refine ih t2.fokker_size ?_ ?_ ?_ rfl ?_ ?_
-                        all_goals grind
-      | abs t => cases t with
-        | bvar _ => grind
-        | fvar _ => grind
-        | app _ _ => grind
-        | abs t =>  intros s hs
-                    unfold subterms at hs
-                    simp at hs
-                    cases hs with
-                    | inl _ => grind
-                    | inr h =>  cases hlc with | abs xs e hlc =>
-                                have ⟨x, _⟩ := fresh_exists <| free_union [fv] String
-                                specialize hlc x (by grind)
-                                cases hlc with | abs ys e hlc =>
-                                have ⟨y, _⟩ := fresh_exists <| free_union [fv] String
-                                specialize hlc y (by grind)
-                                refine @ih ((t⟦0 + 1 ↝ fvar x⟧) ^ fvar y).fokker_size ?_ ((t⟦0 + 1 ↝ fvar x⟧) ^ fvar y) ?_ ?_ ?_ ?_ ?_
-                                any_goals grind
-                                · apply two_vars_are_enough_openRec
-                                  apply two_vars_are_enough_openRec
-                                  grind
-                                · unfold open'
-                                  rw [<- subterms_preserved_under_openRec,
-                                      <- subterms_preserved_under_openRec]
-                                  grind
-                                  grind
-                                  apply two_vars_are_enough_openRec
-                                  grind
+theorem steps_leftmost2_preserves_P_r {fs : Finset (Term String)}
+  (hidempotent : idempotent fs)
+  (h2 :  ∀ t ∈ fs, t.abs_two_vars_are_enough)
+  (hfv : ∀ t ∈ fs, t.fv = ∅)
+  {t t': Term String}
+  (steps : t ↠ℓℓ t')
+  (pt: P fs t):
+  P fs t' := by
+  induction steps with grind [leftmost2_preserves_P_l]
+
+theorem leftmost_rtc_cases {M N}
+  (h : ∀ t', M ↠ℓℓ t' → t'.spine.2.length ≥ 2)
+  (hmn : M ↠ℓ N) : M ↠ℓℓ N \/ ∃ Q, M ↠ℓℓ Q /\ Q ⭢ℓ N := by
+  induction hmn with
+  | refl => grind
+  | tail _ _ ih => cases ih with
+  | inl => grind
+  | inr ih => left
+              obtain ⟨Q, hmq, hqb⟩ := ih
+              refine .tail (by assumption) ?_
+              specialize h _ hmq
+              have h3 := spine_def_2 Q
+              generalize hq : Q.spine.2 = l
+              cases (List.eq_nil_or_concat' l) <;> try grind
+              rename_i heq
+              obtain ⟨L, b, _⟩ := heq
+              subst l
+              rename_i heq
+              rw [heq] at h3
+              rw [List.foldl_concat] at h3
+              cases (List.eq_nil_or_concat' L) <;> try grind
+              rename_i heq
+              obtain ⟨l, b, _⟩ := heq
+              subst L
+              rw [List.foldl_concat] at h3
+              rw [<- h3]
+              rw [<- h3] at hqb
+              constructor <;> assumption
+
+theorem leftmost2_neither_abs_nor_beta_normal {fs : Finset (Term String)}
+  (hidempotent : idempotent fs)
+  (h2 :  ∀ t ∈ fs, t.abs_two_vars_are_enough)
+  (hfv : ∀ t ∈ fs, t.fv = ∅)
+  (t : Term String)
+  (ht : P fs t)
+  (h : ∀ t', t ↠ℓℓ t' → t'.spine.2.length ≥ 2) :
+  ∀ t'', t ↠ℓ t'' → ¬ t''.IsAbs /\ ¬ t''.BetaNormal := by
+  intros t'' g
+  cases (leftmost_rtc_cases h g) with
+  | inl g =>  specialize h _ g
+              have h3 := spine_def_2 t''
+              generalize heq: t''.spine.2 = l
+              rw [heq] at h3 h
+              constructor
+              . grind [IsAbs, BetaNormal]
+              . cases l <;> try grind
+                rename_i l
+                cases l <;> try grind
+                have : GenFinset fs t := by grind
+                have : t.LC := by grind
+                apply normal_app
+                · grind
+                · grind
+                · apply Leftmost2.steps_fv at g
+                  grind
+  | inr g =>  obtain ⟨t', g, g2⟩ := g
+              have : t.fv = ∅ := by grind
+              have : t'.fv = ∅ := by apply Leftmost2.steps_fv at g; grind
+              have : t''.fv = ∅ := by apply BetaAt.step_fv at g2; grind
+              specialize h _ g
+              have h3 := spine_def_2 t'
+              generalize heq: t'.spine.2 = l
+              rw [heq] at h h3
+              cases l <;> try grind
+              rename_i a l
+              cases l <;> try grind
+              rename_i b l
+              rw [<- h3] at g2
+              have : GenFinset fs t := by grind
+              have : P fs t := by grind
+              have : t.LC := by grind
+              have : t'.LC := by grind
+              have : t''.LC := by grind [BetaAt.lc_r]
+              have : t.spine.1 ∈ fs := by grind
+              have := steps_leftmost2_preserves_P_r hidempotent h2 hfv g (by grind)
+              have h3 := h2 t'.spine.1 (by grind)
+              unfold abs_two_vars_are_enough at h3
+              split at h3 <;> try grind
+              rename_i heq
+              rw [heq] at g2
+              rename_i t
+              have : GenFinset fs a := by grind
+              have h4 := leftmost_multiapp t.abs a (b :: l) (by grind) (by grind)
+              have heq := BetaAt.unique h4 g2
+              constructor
+              . induction l using List.reverseRecOn with grind [IsAbs, BetaNormal]
+              . induction l using List.reverseRecOn with
+                | nil =>  intro hnormal
+                          unfold List.foldl at heq
+                          unfold List.foldl at heq
+                          unfold open' openRec at heq
+                          subst t''
+                          apply BetaNormal.app_inv at hnormal
+                          grind
+                | append_singleton l a _ =>
+                          unfold List.foldl at heq
+                          rw [List.foldl_concat] at heq
+                          apply normal_app <;> grind
+
+
+theorem P_progress_to_simple_spine_or_stuck_nonabs {fs : Finset (Term String)}
+  (hidempotent : idempotent fs)
+  (h2 :  ∀ t ∈ fs, t.abs_two_vars_are_enough)
+  (hfv : ∀ t ∈ fs, t.fv = ∅)
+  {t} (ht: P fs t)
+  : (∃ t', t ↠ℓ t' /\ P fs t' /\ (t'.spine.2.length = 0 ∨ t'.spine.2.length = 1)) \/ (∀ t', t ↠ℓ t' -> ¬ IsAbs t' /\ ¬ BetaNormal t') := by
+  cases size_dichotomy t with
+  | inl h => right
+             apply leftmost2_neither_abs_nor_beta_normal hidempotent h2 hfv _ ht h
+  | inr h =>  left
+              obtain ⟨t', h, _⟩ := h
+              refine ⟨t', by grind, steps_leftmost2_preserves_P_r hidempotent h2 hfv h ht, by grind⟩
 
 
 
+theorem exists_leftSpine_reduct {atom : Term String}
+  (h2: atom.abs_two_vars_are_enough)
+  (hfv : atom.fv = ∅)
+  {t}
+  (ht : Gen atom t)
+  (hnormal: Relation.Normalizable Leftmost ((t.app (fvar "x")).app (fvar "y"))) :
+  ∃ t', t ↠ℓ t' /\ P atom.subterms t' /\ (t'.spine.2.length = 0 ∨ t'.spine.2.length = 1) := by
+  have h := @P_progress_to_simple_spine_or_stuck_nonabs atom.subterms subterms_idempotent (subterms_two_vars_are_enough (abs_two_vars_are_enough_weak h2)) (subterms_fv hfv) t ?_
+  cases h with
+  | inl h => grind
+  | inr h =>  exfalso
+              cases normalizable_app_implies_normalizable_or_reduces_to_abs hnormal with
+      | inr h3 => obtain ⟨M, _, g⟩ := h3
+                  cases leftstar_cases g <;> grind
+      | inl h3 => cases normalizable_app_implies_normalizable_or_reduces_to_abs h3 with
+      | inr h3 => grind
+      | inl h3 => obtain ⟨t'', h3, _⟩ := h3
+                  obtain ⟨_, h⟩ := h t'' h3
+                  apply h
+                  rw [betanormal_iff]
+                  sorry
+  rw [<- genfinset_P]
+  apply gen_abs_2_vars_are_enough ht
+  grind
+  apply subterms_two_vars_are_enough (abs_two_vars_are_enough_weak h2)
 
-inductive leftSpine (fs : Finset (Term String)) : Term String → Prop where
-  | singleton : ∀ t ∈ fs, leftSpine fs t
-  | leftApp   : ∀ t1 ∈ fs, ∀ t2, leftSpine fs t2 → leftSpine fs (t1.app t2)
+
+-- this should be trival
+-- I am blocked by next theorems
+theorem exists_leftSpine_reduct2 {fs : Finset (Term String)}
+  (hidempotent : idempotent fs)
+  (h2 :  ∀ t ∈ fs, t.abs_two_vars_are_enough)
+  (hfv : ∀ t ∈ fs, t.fv = ∅)
+  {t} (ht: P fs t)
+  {t head : Term String}
+  (hh : head ∈ fs)
+  (ht : GenFinset fs t)
+  (hnormal: Relation.ReflTransGen Leftmost (((head.app t).app (fvar "x")).app (fvar "y"))
+                                           (((fvar "x").app (fvar "y")).app (H 100))) :
+  ∃ head' t', head' ∈ fs /\ ((head.app t).app (fvar "x")) ↠ℓ head'.app t' /\ P fs t' := by
+  sorry
+-/
 
 end LambdaCalculus.LocallyNameless.Untyped.Term
 
