FokkerChallenge/EnhancedCslib/BetaEtaNormalForm.lean
@@ -4,9 +4,11 @@ import Cslib.Languages.LambdaCalculus.LocallyNameless.Untyped.FullEta
 import Cslib.Languages.LambdaCalculus.LocallyNameless.Untyped.FullBetaConfluence
 import Cslib.Languages.LambdaCalculus.LocallyNameless.Untyped.Congruence
 import Cslib.Languages.LambdaCalculus.LocallyNameless.Untyped.FullBetaEtaConfluence
+import Cslib.Languages.LambdaCalculus.LocallyNameless.Untyped.EtaPostpone
 import FokkerChallenge.EnhancedCslib.CountBvar
 import FokkerChallenge.EnhancedCslib.BetaNormalForm
 import FokkerChallenge.EnhancedCslib.EtaNormalForm
+import FokkerChallenge.EnhancedCslib.Closedunderapp
 import Mathlib.Data.Finset.Lattice.Basic
 
 namespace Cslib
@@ -51,6 +53,85 @@ theorem reflTransGen_iff_eqvGen_of_normal {M N : Term String}
       exact absurd h1 (by decide)
   exact Relation.ChurchRosser.normal_eqvGen_reflTransGen
     (Relation.Confluent.toChurchRosser confluent_beta_eta) norm h
+
+theorem exists_beta_normal_fvar_app_of_beta_eta {Y: Term String} {x} :
+  Relation.Normal FullBetaEta ((fvar x).app Y) ↔ Relation.Normal FullBetaEta Y := by
+  constructor <;> intros h g <;> apply h <;> obtain ⟨M, g⟩ := g
+  . exact ⟨(fvar x).app M, FullBetaEta.step_app_r_cong g (by grind)⟩
+  . cases g <;> rename_i g <;> cases g <;> try grind
+    . rename_i N _ _
+      refine ⟨N, ?_⟩
+      left
+      grind
+    . rename_i g _
+      cases g with | base g => cases g
+    . rename_i N _ _
+      refine ⟨N, ?_⟩
+      right
+      grind
+    . rename_i g _
+      cases g with | base g => cases g
+
+theorem betaeta_nf_fvar {x : String} :
+  Relation.Normal FullBetaEta (fvar x) := by
+  rintro ⟨y, h⟩
+  cases h with
+  | inl h => cases h with | base h => cases h
+  | inr h => cases h with | base h => cases h
+
+
+theorem beta_eta_star_of_beta_normal {M N : Term String} (h : Relation.Normal FullBeta M) (steps : M ↠βηᶠ N) :
+    M ↠ηᶠ N := by
+  induction steps using Relation.ReflTransGen.head_induction_on with
+  | refl => grind
+  | head h' h ih => cases h' with
+    | inl h' => grind
+    | inr h' => exact .head h' (ih (Etastar_normal (.single h') h))
+
+theorem betaeta_nf_app {M N : Term String}
+  (h : ¬ M.IsAbs)
+  (hm : Relation.Normal FullBetaEta M)
+  (hn : Relation.Normal FullBetaEta N) :
+  Relation.Normal FullBetaEta (M.app N) := by
+  rintro ⟨y, h⟩
+  cases h with
+  | inl h => cases h with
+    | base h => cases h with | beta _ _ => grind
+    | appL _ h => apply hn
+                  refine ⟨_, by left; exact h⟩
+    | appR _ h => apply hm
+                  refine ⟨_, by left; exact h⟩
+  | inr h => cases h with
+    | base h => cases h
+    | appL _ h => apply hn
+                  refine ⟨_, by right; exact h⟩
+    | appR _ h => apply hm
+                  refine ⟨_, by right; exact h⟩
+
+
+theorem betaeta_nf_bfvar {M : Term String} (h : M.IsFvar \/ M.IsBvar) :
+  Relation.Normal FullBetaEta M /\ ¬ M.IsAbs := by
+  cases h with
+  | inl h =>  cases h
+              refine ⟨?_, by grind⟩
+              rintro ⟨y, h⟩
+              cases h with
+              | inl h => cases h with | base h => cases h
+              | inr h => cases h with | base h => cases h
+  | inr h =>  cases h
+              refine ⟨?_, by grind⟩
+              rintro ⟨y, h⟩
+              cases h with
+              | inl h => cases h with | base h => cases h
+              | inr h => cases h with | base h => cases h
+
+theorem app_betaeta_nf_bfvar {M : Term String}
+  (h :  ClosedUnderApp (fun t => t.IsFvar \/ t.IsBvar) M) :
+  Relation.Normal FullBetaEta M /\ ¬ M.IsAbs := by
+  induction h with
+  | base _ => grind [betaeta_nf_bfvar]
+  | app _ _ _ _ => exact ⟨betaeta_nf_app (by grind) (by grind) (by grind), by grind⟩
+
 
 end LambdaCalculus.LocallyNameless.Untyped.Term
 
