FokkerChallenge/EnhancedCslib/LeftMost.lean
@@ -1,0 +1,118 @@
+import Cslib.Languages.LambdaCalculus.LocallyNameless.Untyped.Basic
+import Cslib.Languages.LambdaCalculus.LocallyNameless.Untyped.LcAt
+import Cslib.Languages.LambdaCalculus.LocallyNameless.Untyped.LeftmostReduction
+import Cslib.Foundations.Data.HasFresh
+import FokkerChallenge.Basic
+
+namespace Cslib
+
+namespace LambdaCalculus.LocallyNameless.Untyped.Term
+
+theorem Leftmost.induction_rule
+    {motive : ∀ {a b : Term String}, Leftmost a b → Prop}
+    {a b : Term String}
+    (h : Leftmost a b)
+    (h_outer :
+      ∀ (M N : Term String)(hm : M.abs.LC)(hn : N.LC), motive (BetaAt.outer (M:=M) (N:=N) hm hn))
+      (h_appL :
+  ∀ {M M' N : Term String}
+    (h : Leftmost M M')
+    (hi : ¬ IsAbs M),
+    motive h →
+    @motive (M.app N) (M'.app N) (by simpa [Leftmost, hi] using (BetaAt.appL h)))
+      (h_appR :
+  ∀  {M M' N : Term String}
+    (h : Leftmost M M')
+    (hi : ¬ IsAbs N)
+    (g : N.countRedexes = 0),
+    motive h →
+    @motive (N.app M) (N.app M') (by
+      have hidx : (N.countRedexes + if N.IsAbs then 1 else 0) = 0 := by grind
+      unfold Leftmost
+      simpa [hidx] using (@BetaAt.appR _ _ _ _ N h)
+      ))
+    (h_abs :
+      ∀ (M M': Term String) (xs : Finset String)
+        (h :
+          ∀ x ∉ xs,
+            Leftmost (M ^ fvar x) (M' ^ fvar x)),
+      (∀ x hx, motive (h x hx)) →
+      motive (BetaAt.abs xs h))
+    : motive h := by
+  unfold Leftmost at h
+  generalize hi : 0 = i
+  rw [hi] at h
+  induction h with
+  | outer => grind
+  | appL h ih =>
+      rename_i i _ _ _ _
+      have : i = 0 := by omega
+      subst i
+      apply h_appL
+      grind
+      grind
+      exact h
+  | appR h =>
+      rename_i i _ _ _ _ _
+      have : i = 0 := by omega
+      subst i
+      apply h_appR
+      grind
+      grind
+      grind
+      exact h
+  | abs xs h ih =>
+      subst_vars
+      exact h_abs _ _ xs
+        (by
+          intro x hx
+          exact h x hx)
+        (by
+          intro x hx
+          apply ih _ hx
+          omega)
+
+theorem leftmost_multiapp (f a: Term String) (l) : f.abs.LC -> a.LC ->
+  (a :: l).foldl Term.app f.abs ⭢ℓ l.foldl Term.app (f^a) := by
+  induction l using List.reverseRecOn generalizing f a with
+  | nil => apply BetaAt.outer
+  | append_singleton l a _ => intros _ _
+                              simp
+                              apply BetaAt.appNoAbsL
+                              grind
+                              intros h
+                              generalize heq : (List.foldl app (f.abs.app a) l) = Q
+                              rw [heq] at h
+                              cases h
+                              induction l using List.reverseRecOn with grind
+
+theorem leftstar_cases {M N Q : Term String} (h : M.app N ↠ℓ Q) :
+ (∃ M' N', M ↠ℓ M' /\ N ↠ℓ N' /\ Q = M'.app N') \/ ∃ M', M ↠ℓ Term.abs M' :=  by
+  induction h with
+  | refl => grind
+  | tail _ g ih => cases ih with
+    | inr h => grind
+    | inl h => induction g using Leftmost.induction_rule <;> grind
+
+theorem betastar_of_non_abs {M N : Term String} (hm : ∀ M', M ↠ℓ M' -> M'.IsAbs -> False) :
+  ∀ Q, M.app N ↠ℓ Q -> ∃ M' N', M ↠ℓ M' /\ N ↠ℓ N' /\ Q = M'.app N' :=  by
+  grind [leftstar_cases]
+
+theorem normalizable_app_implies_normalizable_or_reduces_to_abs {M N : Term String}
+  (h : Relation.Normalizable Leftmost (Term.app M N)):
+  Relation.Normalizable Leftmost M \/ ∃ M', M'.IsAbs /\ M ↠ℓ M' := by
+  by_contra hcontra
+  simp at hcontra
+  obtain ⟨hm, _⟩ := hcontra
+  obtain ⟨Q, h, g⟩ := h
+  have g_back := g
+  obtain ⟨M', N', hmm', _, _⟩ := @betastar_of_non_abs M N (by grind) Q h
+  apply g_back
+  obtain ⟨M'', h⟩ := hm M' hmm'
+  exists M''.app N'
+  subst Q
+  apply BetaAt.appNoAbsL <;> grind
+
+end LambdaCalculus.LocallyNameless.Untyped.Term
+
+end Cslib
