FokkerChallenge/FamousCombinator.lean
@@ -25,3 +25,78 @@ abs (abs (abs (
   M = λx.x x
 -/
 def M : Term String := abs (app (bvar 0) (bvar 0))
+
+-- H0xy       = x(yy)
+-- H(n + 1)xy = x(y(Hn))
+@[simp, scoped grind =]
+def H : Nat -> Term String
+| 0 => ((bvar 1).app ((bvar 0).app (bvar 0))).abs.abs
+| .succ n => ((bvar 1).app ((bvar 0).app (H n))).abs.abs
+
+@[simp, scoped grind =]
+theorem H_fv {n} : (H n).fv = ∅ := by induction n with grind
+
+@[simp, scoped grind]
+theorem H.LC {n} : (H n).LC := by
+  rw [<- lcAt_iff_LC]
+  induction n with
+  | zero => simp
+  | succ n h => simp
+                exact lcAt_le _ _ _ (by omega) h
+
+theorem normal_H {n} : Relation.Normal FullBetaEta (H n) := by
+  induction n with rw [<- normal_fullBetaEta_iff_no_beta_eta_redex]
+  | zero => decide
+  | succ n h =>
+    left
+    rw [<- normal_fullBetaEta_iff_no_beta_eta_redex] at h
+    refine ⟨?_, ?_⟩
+    . simp [has_beta_redex]
+      cases h with grind [H.LC]
+    . simp [has_eta_redex]
+      cases h with grind [H.LC]
+
+theorem H_succ_reduce {n} : ((H (n + 1)).app (fvar "x")).app (fvar "y") ↠βᶠ ((fvar "x").app ((fvar "y").app (H n))) := by
+    apply Relation.ReflTransGen.head
+    apply Xi.appR
+    grind
+    apply Xi.base
+    apply Beta.beta
+    have : H (n+1) = ((bvar 1).app ((bvar 0).app (H n))).abs.abs := by simp
+    rw [<- this]
+    grind [H.LC]
+    grind
+    refine Relation.ReflTransGen.single (Xi.base ?_)
+    unfold open' openRec openRec openRec
+    rw [openRec_bvar, open_lc]
+    split <;> try grind
+    have : (((fvar "x").app ((bvar 0).app (H n))).open' (fvar "y")) =
+           (((fvar "x").app ((fvar "y").app (H n)))) := by
+      unfold open' openRec openRec
+      rw [openRec_bvar, open_lc]
+      split <;> grind
+      grind [H.LC]
+    rw [<- this]
+    apply Beta.beta
+    apply LC.abs ∅
+    grind [H.LC]
+    grind
+    grind [H.LC]
+
+theorem H_0_reduce : ((H 0).app (fvar "x")).app (fvar "y") ↠βᶠ ((fvar "x").app ((fvar "y").app (fvar "y"))) := by
+    apply Relation.ReflTransGen.head
+    apply Xi.appR
+    grind
+    apply Xi.base
+    apply Beta.beta
+    rw [<- lcAt_iff_LC]
+    decide
+    grind
+    refine .head ((Xi.base (.beta ?_ (by grind)))) ?_
+    unfold openRec openRec openRec
+    split <;> try grind
+    split <;> try grind
+    rw [<- lcAt_iff_LC]
+    decide
+    unfold openRec openRec openRec
+    split <;> grind
