FokkerChallenge/TwoVarsAreNotEnough/Subterms.lean
@@ -1,0 +1,100 @@
+import FokkerChallenge.TwoVarsAreNotEnough.Basic
+import FokkerChallenge.EnhancedCslib.Closedunderapp
+import FokkerChallenge.EnhancedCslib.GenFinset
+
+namespace Cslib
+
+namespace LambdaCalculus.LocallyNameless.Untyped.Term
+
+@[simp, scoped grind =]
+def subterms : Term String -> List (Term String)
+  | Term.bvar _ => []
+  | Term.fvar _ => []
+  | Term.abs (Term.abs t) => t.abs.abs :: (subterms t)
+  | Term.abs _ => []
+  | Term.app t1 t2 => subterms t1 ∪ subterms t2
+
+theorem subterms_subset {t : Term String} :
+    ∀ s ∈ t.subterms, s.subterms ⊆ t.subterms := by
+  induction h : t.fokker_size using Nat.strong_induction_on generalizing t with
+  | h n _ => cases t with (simp_all; try subst_vars)
+  | app _ _ => grind
+  | abs t => cases t with (simp_all; try subst_vars)
+    | abs _ => grind
+
+@[scoped grind]
+theorem subterms_size {t} :
+    ∀ s ∈ subterms t, s.fokker_size <= t.fokker_size := by
+  induction h : t.fokker_size using Nat.strong_induction_on generalizing t with
+  | h n _ => cases t with (simp_all; try subst_vars)
+  | app _ _ => grind
+  | abs t => cases t with (simp_all; try subst_vars)
+    | abs _ => grind
+
+/-
+theorem subterms_gen {t M} (h : Gen t M) : t.subterms = M.subterms := by
+  induction h with grind
+-/
+
+theorem subterms_fv {t} (h : t.fv = ∅) :
+    ∀ s ∈ subterms t, s.fv = ∅ := by
+    induction h : t.fokker_size using Nat.strong_induction_on generalizing t with
+    | h n _ => cases t with  (simp_all; try subst_vars)
+      | app _ _ => grind
+      | abs t => cases t with (simp_all; try subst_vars)
+        | abs _ => grind
+
+theorem subterms_preserved_under_openRec {x i t} (h : two_vars_are_enough t) :
+    t.subterms = t⟦i ↝ fvar x⟧.subterms := by
+    induction h : t.fokker_size using Nat.strong_induction_on generalizing t with
+    | h n _ => cases t with
+    | bvar _ => grind
+    | fvar _ => grind
+    | app _ _ => grind
+    | abs t => cases t with grind
+
+@[scoped grind]
+theorem subterms_two_vars_are_enough {t} (h : two_vars_are_enough t) :
+    ∀ s ∈ subterms t, abs_two_vars_are_enough s := by
+    induction h : t.fokker_size using Nat.strong_induction_on generalizing t with
+    | h n _ => cases t with (simp_all; try subst_vars)
+      | app _ _ => grind
+      | abs t => cases t with (simp_all; try subst_vars)
+        | abs _ => grind
+
+theorem two_vars_are_enough_subterms_lc {t} (h : two_vars_are_enough t) :
+    ∀ s ∈ subterms t, s.LC := by grind
+
+theorem subterms_closedunderappbool {t} (h : ClosedUnderAppBool abs_two_vars_are_enough t) :
+    ∀ s ∈ subterms t, abs_two_vars_are_enough s := by
+    induction h : t.fokker_size using Nat.strong_induction_on generalizing t with
+    | h n _ => cases t with (simp_all; try subst_vars)
+      | app _ _ => grind
+      | abs t => cases t with (simp_all; try subst_vars)
+        | abs _ => grind
+
+theorem closedUnderAppBool_genfinset_subterms {t}
+    (h : ClosedUnderAppBool abs_two_vars_are_enough t) :
+    GenFinset t.subterms t := by
+  induction ht : t.fokker_size using Nat.strong_induction_on generalizing t with | h n ih =>
+  cases t with
+  | bvar _ => cases h
+  | fvar _ => cases h
+  | abs t => cases t <;> grind
+  | app x y =>  have hx := @ih x.fokker_size (by grind) x (by grind) rfl
+                have hy := @ih y.fokker_size (by grind) y (by grind) rfl
+                refine .app (genfinset_subset (by grind) hx) (genfinset_subset (by grind) hy)
+
+/-
+@[scoped grind =]
+def idempotent (terms : Finset (Term String)) : Prop :=
+  terms.biUnion subterms = terms
+
+theorem subterms_idempotent {t : Term String} : idempotent t.subterms := by
+    induction h : t.fokker_size using Nat.strong_induction_on generalizing t with
+    | h n _ => cases t with
+    | bvar _ => grind
+    | fvar _ => grind
+    | app _ _ => grind
+    | abs t => cases t with grind
+-/
