FokkerChallenge/TwoVarsAreNotEnough/U.lean
@@ -1,0 +1,362 @@
+import Cslib.Languages.LambdaCalculus.LocallyNameless.Untyped.Basic
+import Cslib.Languages.LambdaCalculus.LocallyNameless.Untyped.LcAt
+import Cslib.Languages.LambdaCalculus.LocallyNameless.Untyped.ListFullBeta
+import Cslib.Languages.LambdaCalculus.LocallyNameless.Untyped.FullBetaConfluence
+import Cslib.Languages.LambdaCalculus.LocallyNameless.Untyped.LeftmostReduction
+import Cslib.Foundations.Data.HasFresh
+import FokkerChallenge.Basic
+import FokkerChallenge.FamousCombinator
+import FokkerChallenge.EnhancedCslib.Basic
+import FokkerChallenge.EnhancedCslib.FlipApp
+import FokkerChallenge.EnhancedCslib.LeftMost
+import FokkerChallenge.EnhancedCslib.BetaNormalForm
+import FokkerChallenge.EnhancedCslib.Closedunderapp
+import FokkerChallenge.EnhancedCslib.List
+import FokkerChallenge.EnhancedCslib.ReflTransGenWithSteps
+import FokkerChallenge.EnhancedCslib.HeadRed
+import FokkerChallenge.TwoVarsAreNotEnough.Basic
+import FokkerChallenge.TwoVarsAreNotEnough.Head2
+import FokkerChallenge.TwoVarsAreNotEnough.Unroll
+import Mathlib.Data.Finset.Basic
+import Mathlib.Data.Finset.Insert
+import Mathlib.Data.Finset.Union
+
+namespace Cslib
+
+namespace LambdaCalculus.LocallyNameless.Untyped.Term
+
+@[scoped grind]
+def U (n : Nat) (x z : String) (a: Term String) : Prop :=
+  a = fvar x \/
+  (a.abs_two_vars_are_enough /\ a.depth < n) \/
+  ∃ l : List _, a = l.foldl (flip app) (fvar z) /\ ∀ x ∈ l, x.abs_two_vars_are_enough /\ x.depth <= n
+
+theorem U.LC {n x z }: ∀ N, U n x z N -> N.LC := by
+  intros N h
+  rcases h with _|_|⟨l, _, _⟩
+  . grind
+  . grind
+  . subst_vars
+    rw [flip_app_lc]
+    grind
+
+theorem two_vars_are_enough_openRec_U {n t N1 N0 x z}
+  (g : two_vars_are_enough t)
+  (ht : t.depth < n)
+  (h1: ClosedUnderApp (U n x z) N1)
+  (h2: ClosedUnderApp (U n x z) N0) :
+  ClosedUnderApp (U n x z) (t⟦1 ↝ N1⟧⟦0 ↝ N0⟧) := by
+  induction t with
+  | fvar _ => grind
+  | app _ _ iha ihb =>  simp at ht
+                        exact .app (iha (by grind) (by grind)) (ihb (by grind) (by grind))
+  | abs t => cases t with
+    | abs _ => grind
+    | bvar _ => unfold two_vars_are_enough at g
+                grind
+    | fvar _ => unfold two_vars_are_enough at g
+                grind
+    | app _ _ =>  unfold two_vars_are_enough at g
+                  grind
+  | bvar a => unfold two_vars_are_enough at g
+              have h : a = 0 \/ a = 1 := by grind
+              cases h <;> subst_vars
+              . grind
+              . simp [openRec]
+                rw [open_lc]
+                . grind
+                . apply closedunderapp_lc U.LC h1
+
+theorem HeadReduction2_step_preserve_closedUnderApp_U {M N n x z}
+  (hmn: HeadReduction2 M N)
+  (hm : ClosedUnderApp (U n x z) M) :
+  ClosedUnderApp (U n x z) N  := by
+  induction hmn with
+  | appL h _ => cases hm with
+    | app => grind
+    | base hm =>  rcases hm with _|_|⟨l, hl, g⟩
+                  . grind
+                  . grind
+                  . rcases (List.eq_nil_or_concat' l) with _| ⟨l, b, h⟩
+                    . grind
+                    . subst_vars
+                      rw [List.foldl_concat] at hl
+                      unfold flip at hl
+                      cases hl
+                      rename_i M _ _
+                      specialize g M (by grind)
+                      cases h <;> grind
+  | base => cases hm with
+    | base hm =>  rcases hm with _|⟨_, _⟩|⟨l, hl, g⟩
+                  . grind
+                  . grind
+                  . rcases (List.eq_nil_or_concat' l) with _| ⟨l, b, h⟩
+                    . grind
+                    . subst_vars
+                      rw [List.foldl_concat] at hl
+                      unfold flip at hl
+                      cases hl
+                      rename_i M N
+                      specialize g (M.abs.abs.app N) (by grind)
+                      grind
+    | app hm _ => cases hm with
+      | app hm _ => cases hm with | base hm =>
+                    rcases hm with _|_|⟨l, hl, h⟩
+                    . grind
+                    . apply two_vars_are_enough_openRec_U <;> grind
+                    . rcases (List.eq_nil_or_concat' l) with _| ⟨l, b, h⟩
+                      . grind
+                      . subst_vars
+                        rw [List.foldl_concat] at hl
+                        unfold flip at hl
+                        cases hl
+      | base hm =>  rcases hm with _|⟨_, _⟩|⟨l, hl, g⟩
+                    . grind
+                    . grind
+                    . rcases (List.eq_nil_or_concat' l) with _| ⟨l, b, h⟩
+                      . grind
+                      . subst_vars
+                        rw [List.foldl_concat] at hl
+                        unfold flip at hl
+                        cases hl
+                        rename_i M _ _
+                        apply two_vars_are_enough_openRec_U
+                        . specialize g M.abs.abs (by grind)
+                          grind
+                        . specialize g M.abs.abs (by grind)
+                          grind
+                        . refine .base ?_
+                          right
+                          right
+                          refine ⟨l, ?_, by grind⟩
+                          unfold flip
+                          grind
+                        . grind
+
+theorem HeadReduction2_steps_preserve_closedUnderApp_U {M N n x z}
+  (steps : M ↠𝒽 N)
+  (hm : ClosedUnderApp (U n x z) M) :
+  ClosedUnderApp (U n x z) N  := by
+  induction steps with grind [HeadReduction2_step_preserve_closedUnderApp_U]
+
+
+theorem closedUnderApp_reduce_to_head_apps (x z n) {M N}
+  (hxz : x ≠ z)
+  (hm : ClosedUnderApp (U n x z) M)
+  (hx : x ∈ N.fv)
+  (hmn : unroll M N) :
+  ∃ l: List _, M ↠βᶠ l.foldl (flip app) N /\
+               ∀ x ∈ l, x.abs_two_vars_are_enough /\ x.depth < n := by
+  induction hmn using Relation.ReflTransGen.head_induction_on with
+  | refl => exact ⟨[], by grind⟩
+  | head h' h ih => cases h' with
+  | reflTrans h' =>
+  obtain ⟨l, ih, _⟩ := ih (HeadReduction2_step_preserve_closedUnderApp_U h' hm)
+  exact ⟨l, .trans (HeadReduction2.step_2_beta h' (closedunderapp_lc U.LC hm)) ih, by grind⟩
+  | throughAbsApp => cases hm with
+    | app hn hc => cases hn with | base hn =>
+        specialize ih hc
+        rcases hn with _|_|⟨l, hl, _⟩
+        . grind
+        . rename_i Z _
+          obtain ⟨l, ih, _⟩ := ih
+          refine ⟨l ++ [Z.abs], ?_, by grind⟩
+          rw [List.foldl_concat]
+          unfold flip
+          apply FullBeta.redex_app_r_cong ih (by grind)
+        . rcases (List.eq_nil_or_concat' l) with _| ⟨l, b, h⟩
+          . grind
+          . subst_vars
+            rw [List.foldl_concat] at hl
+            unfold flip at hl
+            grind
+    | base hm =>  rcases hm with _|⟨hm, _⟩|⟨l, heq, _⟩
+                  . grind
+                  . cases hm
+                  . exfalso
+                    have g := congrArg fv heq
+                    have h5 : ∀ x ∈ l, x.fv = ∅ := by grind
+                    rw [<- List.map_eq_replicate_iff] at h5
+                    rw [flip_app_fv, h5, foldl_union_replicate_empty] at g
+                    apply unroll.fv at h
+                    specialize h hx
+                    have : x ∈ ({z} : Finset String) := by grind
+                    grind
+
+theorem U_le_fvar_or_combinator{i y z} : U i y z ≤ ClosedUnderApp fvar_or_combinator := by
+  intro x hx
+  rcases hx with _|_|⟨l, h, _⟩
+  . grind
+  . grind
+  . subst x
+    induction l using List.reverseRecOn with
+    | nil => grind
+    | append_singleton l a _ =>
+    rw [List.foldl_concat]
+    simp [flip]
+    exact .app (by grind) (by grind)
+
+theorem U_replicate {n x z i M} :
+  ClosedUnderApp (U n x z) M ->
+  ClosedUnderApp (U n x z) (List.foldl app M (List.replicate i (fvar x))) := by
+  induction i generalizing M with grind
+
+theorem U_foldl_z {Z l n x z}
+  (h : ClosedUnderApp (U n x z) (List.foldl app (fvar z) (Z :: l))):
+  ClosedUnderApp (U n x z) Z := by
+  induction l using List.reverseRecOn with
+  | nil =>  simp_all
+            cases h with
+            | app _ _ => grind
+            | base h => rcases h with _|_|⟨l, h, hl⟩
+                        . grind
+                        . grind
+                        . exfalso
+                          induction l using List.reverseRecOn with
+                          | nil => simp_all
+                          | append_singleton l a _ =>
+                          simp_all [flip]
+                          obtain ⟨_, h⟩ := h
+                          subst_vars
+                          specialize hl (fvar z) (by grind)
+                          grind
+  | append_singleton l a _ =>
+  simp at h
+  cases h with
+  | app _ _ => grind
+  | base h => rcases h with _|_|⟨l, h, hl⟩
+              . grind
+              . grind
+              . exfalso
+                induction l using List.reverseRecOn with
+                | nil => simp_all
+                | append_singleton _ a _ =>
+                simp_all [flip]
+                obtain ⟨_, h⟩ := h
+                subst_vars
+                obtain ⟨_, _⟩ := hl (List.foldl app ((fvar z).app Z) l) (by grind)
+                induction l  using List.reverseRecOn with grind
+
+theorem U_foldl_x {Z l n x z}
+  (h : ClosedUnderApp (U n x z) (List.foldl app (fvar x) (Z :: l))):
+  ClosedUnderApp (U n x z) Z := by
+  induction l using List.reverseRecOn with
+  | nil =>  simp_all
+            cases h with
+            | app _ _ => grind
+            | base h => rcases h with _|_|⟨l, h, hl⟩
+                        . grind
+                        . grind
+                        . exfalso
+                          induction l using List.reverseRecOn with
+                          | nil => simp_all
+                          | append_singleton l a _ =>
+                          simp_all [flip]
+                          obtain ⟨_, h⟩ := h
+                          subst_vars
+                          specialize hl (fvar x) (by grind)
+                          grind
+  | append_singleton l a _ =>
+  simp at h
+  cases h with
+  | app _ _ => grind
+  | base h => rcases h with _|_|⟨l, h, hl⟩
+              . grind
+              . grind
+              . exfalso
+                induction l using List.reverseRecOn with
+                | nil => simp_all
+                | append_singleton _ a _ =>
+                simp_all [flip]
+                obtain ⟨_, h⟩ := h
+                subst_vars
+                obtain ⟨_, _⟩ := hl (List.foldl app ((fvar x).app Z) l) (by grind)
+                induction l  using List.reverseRecOn with grind
+
+theorem U_subst_x {n x z y M} (h : (U n x z) M) (hxz : x ≠ z) :
+  (U n y z) M[x:=fvar y] := by
+  rcases h with _|_|⟨l, h, _⟩
+  . grind
+  . rw [subst_fresh] <;> grind
+  . right
+    right
+    refine ⟨l, ?_, by grind⟩
+    subst M
+    rw [subst_fresh]; try grind
+    rw [flip_app_fv]
+    have h5 : ∀ x ∈ l, x.fv = ∅ := by grind
+    rw [<- List.map_eq_replicate_iff] at h5
+    rw [h5, foldl_union_replicate_empty]
+    grind
+
+theorem U_subst_x_closedunderapp (y) {n x z M} (hxz : x ≠ z) (h : ClosedUnderApp (U n x z) M):
+  ClosedUnderApp (U n y z) M[x:=fvar y] := by
+  induction h with grind [U_subst_x]
+
+theorem U_subst_z {n x z y M} (h : (U n x z) M) (hxz : x ≠ z) :
+  (U n x y) M[z:=fvar y] := by
+  rcases h with _|_|⟨l, h, _⟩
+  . grind
+  . rw [subst_fresh] <;> grind
+  . right
+    right
+    refine ⟨l, ?_, by grind⟩
+    subst M
+    rw [multiapp_subst, subst_fvar]
+    split <;> try grind
+    apply congr rfl
+    induction l with
+    | nil => grind
+    | cons head tail ih =>  simp
+                            rw [subst_fresh] <;> grind
+
+theorem U_subst_z_closedunderapp (y) {n x z M} (hxz : x ≠ z) (h : ClosedUnderApp (U n x z) M):
+  ClosedUnderApp (U n x y) M[z:=fvar y] := by
+  induction h with grind [U_subst_z]
+
+theorem U_fv {n x z M}  (h : U n x z M): M.fv ⊆ {x, z} := by
+  rcases h with _|_|⟨l, h, _⟩
+  . grind
+  . grind
+  . subst_vars
+    rw [flip_app_fv]
+    have h5 : ∀ x ∈ l, x.fv = ∅ := by grind
+    rw [<- List.map_eq_replicate_iff] at h5
+    rw [h5, foldl_union_replicate_empty]
+    grind
+
+theorem app_U_fv {n x z M} (h : ClosedUnderApp (U n x z) M):
+   M.fv ⊆ {x, z} := by
+   induction h with grind [U_fv]
+
+theorem U_transform (x) {n z} : U n z z ≤ U n x z := by
+  intros M h
+  rcases h with _|_|⟨l, h, _⟩
+  . right
+    right
+    use []
+    grind
+  . grind
+  . grind
+
+theorem app_U_transform (x) {n z} : ClosedUnderApp (U n z z) ≤ ClosedUnderApp (U n x z) := by
+  intros M h
+  induction h with
+  | base h => exact .base (U_transform _ _ h)
+  | app _ _ _ _ => grind
+
+theorem U0 {x y} : U 0 x y ≤ (fun t => t.IsFvar \/ t.IsBvar) := by
+  intros M h
+  rcases h with _|_|⟨l, h, hl⟩
+  . grind
+  . grind
+  . cases l with
+    | nil => grind
+    | cons head tail => specialize hl head (by grind)
+                        grind
+
+theorem app_U0 {x y} : ClosedUnderApp (U 0 x y) ≤ ClosedUnderApp (fun t => t.IsFvar \/ t.IsBvar) := by
+  intros M h
+  induction h with
+  | base h => exact .base (U0 _ h)
+  | app _ _ _ _ => grind
